Test/tutorial/ImpVerifiedCompiler/comparison/IMP.dfy
@@ -3,54 +3,49 @@ include "Sequences.dfy"
 type ident = string
 
 datatype aexp =
-	| AConst(int)
-	| AId(ident)
-	| APlus(aexp, aexp)
-	| AMinus(aexp, aexp)
-
-datatype bexp =
-	| BTrue
-	| BFalse
-	| BEq(aexp, aexp)
-	| BLe(aexp, aexp)
-	| BNot(bexp)
-	| BAnd(bexp, bexp)
-
-datatype com =
-	| CSkip
-	| CAsgn(ident, aexp)
-	| CSeq(com, com)
-	| CIf(bexp, com, com)
-	| CWhile(bexp, com)
-
-type store = map<ident,int>
+	| CONST(n: int)
+	| VAR(x: ident)
+	| PLUS(a1: aexp, a2: aexp)
+	| MINUS(a1: aexp, a2: aexp)
 
 predicate id_in_aexp(id: ident, a: aexp) {
 	match a
-		case AConst(n) => false
-		case AId(id') => id == id'
-		case APlus(a1, a2) => id_in_aexp(id,a1) || id_in_aexp(id,a2)
-		case AMinus(a1, a2) => id_in_aexp(id,a1) || id_in_aexp(id,a2)
+		case CONST(n) => false
+		case VAR(id') => id == id'
+		case PLUS(a1, a2) => id_in_aexp(id,a1) || id_in_aexp(id,a2)
+		case MINUS(a1, a2) => id_in_aexp(id,a1) || id_in_aexp(id,a2)
 }
 	
 function aeval(s: store, a: aexp): int
 	requires forall id: ident :: id_in_aexp(id,a) ==> id in s
 {
 	match a
-		case AConst(n) => n
-		case AId(id) => s[id]
-		case APlus(a1, a2) => aeval(s,a1) + aeval(s,a2)
-		case AMinus(a1, a2) => aeval(s,a1) - aeval(s,a2)
+		case CONST(n) => n
+		case VAR(id) => s[id]
+		case PLUS(a1, a2) => aeval(s,a1) + aeval(s,a2)
+		case MINUS(a1, a2) => aeval(s,a1) - aeval(s,a2)
 }
+
+/* Examples of evaluation */
+
+/* aeval_free */
 	
+datatype bexp =
+	| TRUE
+	| FALSE
+	| EQUAL(a1: aexp, a2: aexp)
+	| LESSEQUAL(a1: aexp, a2: aexp)
+	| NOT(b1: bexp)
+	| AND(b1: bexp, b2: bexp)
+
 predicate id_in_bexp(id: ident, b: bexp) {
 	match b
-		case BTrue => true
-		case BFalse => false
-		case BEq(a1,a2) => id_in_aexp(id,a1) || id_in_aexp(id,a2)
-		case BLe(a1,a2) => id_in_aexp(id,a1) || id_in_aexp(id,a2)
-		case BNot(b) => id_in_bexp(id,b)
-		case BAnd(b1,b2) => id_in_bexp(id,b1) || id_in_bexp(id,b2)
+		case TRUE => true
+		case FALSE => false
+		case EQUAL(a1,a2) => id_in_aexp(id,a1) || id_in_aexp(id,a2)
+		case LESSEQUAL(a1,a2) => id_in_aexp(id,a1) || id_in_aexp(id,a2)
+		case NOT(b) => id_in_bexp(id,b)
+		case AND(b1,b2) => id_in_bexp(id,b1) || id_in_bexp(id,b2)
 			
 }
 	
@@ -58,44 +53,57 @@ function beval(s: store, b: bexp): bool
 	requires forall id: ident :: id_in_bexp(id,b) ==> id in s
 {
 	match b
-		case BTrue => true
-		case BFalse => false
-		case BEq(a1, a2) => aeval(s,a1) == aeval(s,a2)
-		case BLe(a1, a2) => aeval(s,a1) <= aeval(s,a2)
-		case BNot(b) => ! beval(s,b)
-		case BAnd(b1,b2) => beval(s,b1) && beval(s,b2)
+		case TRUE => true
+		case FALSE => false
+		case EQUAL(a1, a2) => aeval(s,a1) == aeval(s,a2)
+		case LESSEQUAL(a1, a2) => aeval(s,a1) <= aeval(s,a2)
+		case NOT(b) => ! beval(s,b)
+		case AND(b1,b2) => beval(s,b1) && beval(s,b2)
 }
-	
+
+/* Derived forms */
+
+datatype com =
+	| SKIP
+	| ASSIGN(x: ident, a: aexp)
+	| SEQ(c1: com, c2: com)
+	| IFTHENELSE(b: bexp, c1: com, c2: com)
+	| WHILE(b: bexp, c1: com)
+
 predicate id_in_com(id: ident, c: com) {
 	match c
-		case CSkip => false
-		case CAsgn(id',a) => id_in_aexp(id,a) 
-		case CSeq(c1, c2) => id_in_com(id,c1) || id_in_com(id,c2)
-		case CIf(b,c1,c2) => id_in_bexp(id,b) || id_in_com(id,c1) || id_in_com(id,c2)
-		case CWhile(b,c) => id_in_bexp(id,b) || id_in_com(id,c)
+		case SKIP => false
+		case ASSIGN(id',a) => id_in_aexp(id,a) 
+		case SEQ(c1, c2) => id_in_com(id,c1) || id_in_com(id,c2)
+		case IFTHENELSE(b,c1,c2) => id_in_bexp(id,b) || id_in_com(id,c1) || id_in_com(id,c2)
+		case WHILE(b,c) => id_in_bexp(id,b) || id_in_com(id,c)
 }
 	
+type store = map<ident,int>
+
 least predicate cexec(s1: store, c: com, s2: store)
 {
 	match c
-		case CSkip => s1 == s2
-		case CAsgn(id,a) =>
+		case SKIP => s1 == s2
+		case ASSIGN(id,a) =>
 			if (forall id: ident :: id_in_aexp(id,a) ==> id in s1) then s2 == s1[id := aeval(s1,a)] else false
-		case CSeq(c1, c2) => exists si: store :: cexec(s1,c1,si) && cexec(si,c2,s2)
-		case CIf(b,c1,c2) =>
+		case SEQ(c1, c2) => exists si: store :: cexec(s1,c1,si) && cexec(si,c2,s2)
+		case IFTHENELSE(b,c1,c2) =>
 			if (forall id: ident :: id_in_bexp(id,b) ==> id in s1) then 
 			(if beval(s1,b) then cexec(s1,c1,s2) else cexec(s1,c2,s2))
 			else false
-		case CWhile(b,c) =>
+		case WHILE(b,c) =>
 			if (forall id: ident :: id_in_bexp(id,b) ==> id in s1) then 
-			if beval(s1,b) then (exists si: store :: cexec(s1,c,si) && cexec(si,CWhile(b,c),s2)) else s1 == s2
+			if beval(s1,b) then (exists si: store :: cexec(s1,c,si) && cexec(si,WHILE(b,c),s2)) else s1 == s2
 			else false
 }
 
+/* Missing cexec_infinite_loop and cexec_Bounded */
+
 datatype cont =
   | Kstop
-	| Kseq(com,cont)
-	| Kwhile(bexp,com,cont)
+	| Kseq(c: com,k: cont)
+	| Kwhile(b: bexp, c: com, k: cont)
 
 type conf = (com,cont,store)
 
@@ -103,41 +111,43 @@ predicate step(conf1: conf, conf2: conf) {
 	var (c1,k1,s1) := conf1;
 	var (c2,k2,s2) := conf2;
 	match (c1,k1) {
-		case (CAsgn(i, a), _) =>
+		case (ASSIGN(i, a), _) =>
 			&& (forall id: ident :: id_in_aexp(id,a) ==> id in s1)
-			&& c2 == CSkip
+			&& c2 == SKIP
 			&& k2 == k1
 			&& s2 == s1[i := aeval(s1,a)]
-		case (CSeq(c1', c1''), k) =>
+		case (SEQ(c1', c1''), k) =>
 			&& c2 == c1'
 			&& k2 == Kseq(c1'',k)
 			&& s2 == s1
-		case (CIf(b, cifso, cifnotso), _) =>
+		case (IFTHENELSE(b, cifso, cifnotso), _) =>
 			&& (forall id: ident :: id_in_bexp(id,b) ==> id in s1)
 			&& c2 == (if beval(s1, b) then cifso else cifnotso)
 			&& k2 == k1
 			&& s2 == s1
-		case (CWhile(b, c), k) =>
+		case (WHILE(b, c), k) =>
 			&& (forall id: ident :: id_in_bexp(id,b) ==> id in s1)
-			&& c2 == (if beval(s1,b) then c else CSkip)
+			&& c2 == (if beval(s1,b) then c else SKIP)
 			&& k2 == (if beval(s1,b) then Kwhile(b,c,k) else k1)
 			&& s2 == s1
-		case (CSkip, Kseq(c, k)) =>
+		case (SKIP, Kseq(c, k)) =>
 			&& c2 == c
 			&& k2 == k
 			&& s2 == s1
-		case (CSkip, Kwhile(b, c, k)) =>
-			&& c2 == CWhile(b,c)
+		case (SKIP, Kwhile(b, c, k)) =>
+			&& c2 == WHILE(b,c)
 			&& k2 == k
 			&& s2 == s1
 		case _ => false
 	}
 }
 
+/*
 predicate fin_reds(conf1: conf, conf2: conf) {
 	star((c1,c2) => step(c1,c2),conf1,conf2)
 }
 	
 predicate inf_reds(conf: conf) {
-	inf((c1,c2) => step(c1,c2),conf)
+	infseq((c1,c2) => step(c1,c2),conf)
 }
+*/
