Test/tutorial/ImpVerifiedCompiler/comparison/Sequences.dfy
@@ -2,10 +2,6 @@ least predicate star<T(!new)>(R: (T,T) -> bool, conf1: T, conf2: T) {
 	(conf1 == conf2) || (exists conf_inter: T :: R(conf1, conf_inter) && star(R,conf_inter, conf2))
 }
 
-predicate Star<T(!new)>(R: (T,T) -> bool, conf1: T, conf2: T) {
-  star(R, conf1, conf2)
-}
-
 lemma star_one_sequent<T(!new)>(R: (T,T) -> bool, conf1: T, conf2: T)
 	requires R(conf1,conf2)
 	ensures star(R,conf1,conf2)
@@ -15,6 +11,10 @@ lemma star_one_sequent<T(!new)>(R: (T,T) -> bool, conf1: T, conf2: T)
 lemma star_one<T(!new)>()
 	ensures forall R: (T,T) -> bool :: forall conf1, conf2: T :: R(conf1,conf2) ==> star(R,conf1,conf2)
 {
+}
+
+predicate Star<T(!new)>(R: (T,T) -> bool, conf1: T, conf2: T) {
+  star(R, conf1, conf2)
 }
 
 least lemma star_trans_pre<T(!new)>(R: (T,T) -> bool, conf1: T, conf2: T, conf3: T)
@@ -47,14 +47,6 @@ lemma star_trans<T(!new)>()
 	}
 }
 
-lemma combine_reductions<T(!new)>()
-	ensures forall R: (T,T) -> bool :: forall conf1, conf2: T :: R(conf1,conf2) ==> star(R,conf1,conf2)
-	ensures forall R: (T,T) -> bool :: forall conf1, conf2, conf3: T :: (star(R,conf1,conf2) && star(R,conf2,conf3)) ==> star(R,conf1,conf3)
-{
-	star_one<T>();
-	star_trans<T>();
-}
-
 least predicate plus<T(!new)>(R: (T,T) -> bool, conf1: T, conf2: T) {
 	(exists conf_inter: T :: R(conf1, conf_inter) && star(R,conf_inter, conf2))
 }
@@ -78,6 +70,8 @@ lemma plus_star<T(!new)>(R: (T,T) -> bool, conf1: T, conf2: T)
 	star_trans_sequent(R,conf1,conf1',conf2);
 }
 
+/* Missing plus_star_trans */
+
 lemma star_plus_trans<T(!new)>(R: (T,T) -> bool, conf1: T, conf2: T, conf3: T)
 	requires star(R,conf1,conf2)
 	requires plus(R,conf2,conf3)
@@ -93,23 +87,30 @@ lemma star_plus_trans<T(!new)>(R: (T,T) -> bool, conf1: T, conf2: T, conf3: T)
 	}
 }
 
+/* Missing plus_right */
+
+/* Missing irred */
 
 predicate all_seq_inf<T(!new)>(R: (T,T) -> bool,conf: T) {
 	forall conf2: T :: star(R,conf,conf2) ==> exists conf3: T :: R(conf2,conf3)
 }
 
-greatest predicate inf<T(!new)>(R: (T,T) -> bool,conf: T) {
-	exists confi: T :: R(conf,confi) && inf(R,confi)
+/* Missing infseq_with_function */
+
+greatest predicate infseq<T(!new)>(R: (T,T) -> bool,conf: T) {
+	exists confi: T :: R(conf,confi) && infseq(R,confi)
 }
 
 greatest predicate Inf<T(!new)>(R: (T,T) -> bool,conf: T) {
-	inf(R,conf)
+	infseq(R,conf)
 }
+
+/* Missing cycle_infseq */
 
 least lemma star_inf_trans<T(!new)>(R: (T,T) -> bool, conf1: T, conf2: T)
 	requires star(R,conf1,conf2)
-	requires inf(R,conf2)
-	ensures inf(R,conf1)
+	requires infseq(R,conf2)
+	ensures infseq(R,conf1)
 {
 	if conf1 == conf2 {}
 	else {
@@ -120,17 +121,17 @@ least lemma star_inf_trans<T(!new)>(R: (T,T) -> bool, conf1: T, conf2: T)
 	
 greatest lemma infseq_if_all_seq_inf_pre<T(!new)>(R: (T,T) -> bool, conf: T)
 	requires forall conf2: T :: star(R,conf,conf2) ==> exists conf3: T :: R(conf2,conf3)
-	ensures inf(R,conf)
+	ensures infseq(R,conf)
 {
 	assert star(R,conf,conf);
 	var B :| R(conf,B);
 	assert R(conf,B);
-	assert inf(R,B) by { infseq_if_all_seq_inf_pre(R,B); }
+	assert infseq(R,B) by { infseq_if_all_seq_inf_pre(R,B); }
 }
 
 lemma infseq_if_all_seq_inf<T(!new)>(R: (T,T) -> bool, conf: T)
 	requires all_seq_inf(R,conf)
-	ensures inf(R,conf)
+	ensures infseq(R,conf)
 {
 	infseq_if_all_seq_inf_pre(R,conf);
 }
@@ -138,7 +139,7 @@ lemma infseq_if_all_seq_inf<T(!new)>(R: (T,T) -> bool, conf: T)
 lemma infseq_coinduction_principle_ord<T(!new)>(k: ORDINAL, R: (T,T) -> bool, X: T -> bool, a : T)
 	requires (forall a: T :: X(a) ==> exists b: T :: R(a,b) && X(b))
 	requires X(a)
-	ensures inf#[k](R,a)
+	ensures infseq#[k](R,a)
 {
 	if k.Offset == 0 {} else {
 		var b :| R(a,b) && X(b);
@@ -152,10 +153,10 @@ predicate {:opaque} always_step<T(!new)>(R: (T,T) -> bool, X: T -> bool) {
 
 greatest lemma infseq_coinduction_principle_pre<T(!new)>(R: (T,T) -> bool, X: T -> bool, a: T)
 	requires always_step(R,X)
-	ensures  X(a) ==> inf(R,a)
+	ensures  X(a) ==> infseq(R,a)
 {
 	reveal always_step();
-	forall a: T ensures X(a) ==> inf(R,a) {
+	forall a: T ensures X(a) ==> infseq(R,a) {
 		if X(a) {
 			var b :| R(a,b) && X(b);
 			infseq_coinduction_principle_pre(R,X,a);
@@ -166,7 +167,7 @@ greatest lemma infseq_coinduction_principle_pre<T(!new)>(R: (T,T) -> bool, X: T 
 lemma infseq_coinduction_principle<T(!new)>(R: (T,T) -> bool, X: T -> bool, a : T)
 	requires always_step(R,X)
 	requires X(a)
-	ensures inf(R,a)
+	ensures infseq(R,a)
 {
 	reveal always_step();
 	if X(a) {
@@ -200,7 +201,7 @@ lemma infseq_coinduction_principle_2_pre_lift<T(!new)>(R: (T,T) -> bool, X: T ->
 lemma infseq_coinduction_principle_2<T(!new)>(R: (T,T) -> bool, X: T -> bool, a : T)
 	requires H1: always_steps(R,X)
 	requires H2: X(a)
-	ensures inf(R,a)
+	ensures infseq(R,a)
 {
 
 	assert Y(R,X,a) by {
@@ -216,3 +217,6 @@ lemma infseq_coinduction_principle_2<T(!new)>(R: (T,T) -> bool, X: T -> bool, a 
 	infseq_coinduction_principle(R,(a: T) => Y(R,X,a),a);
 	
 }
+
+/* The tutorial continues from there */
+
